src/Pipeline.v
@@ -1,0 +1,83 @@
+Require Import Coq.Lists.List.
+Import ListNotations.
+Require Import lib.LibTacticsMin.
+Require Import bbv.Word.
+Require Import compiler.Decidable.
+Require Import compiler.Op.
+Require Import compiler.ResMonad.
+Require        compiler.ExprImp.
+Require Import compiler.FlattenExpr.
+Require        compiler.FlatImp.
+Require        compiler.FlatToRiscv.
+Require Import compiler.Riscv.
+Require Import compiler.Machine.
+Require Import compiler.StateMonad.
+Require Import compiler.runsToSatisfying.
+Require Import compiler.MyOmega.
+Require Import compiler.zcast.
+Require Import compiler.NameGen.
+Require Import compiler.Common.
+
+Section Pipeline.
+
+  Context {wlit: nat}. (* max bit width of literals *)
+  Context {wdiff: nat}. (* difference between literal width and word width *)
+  Context {wjimm: nat}.
+  Notation w := (wlit + wdiff).
+  Variable w_lbound: w >= wjimm.
+  Variable wlit_bound: 2 <= wlit <= wjimm.
+  Variable wjimm_bound: 2 <= wjimm <= w.
+  Context {var: Set}.
+  Context {eq_var_dec: DecidableEq var}.
+  Context {state: Type}.
+  Context {stateMap: Map state var (word w)}.
+  Context {vars: Type}.
+  Context {varset: set vars var}.
+  Context {NGstate: Type}.
+  Context {NG: NameGen var vars NGstate}.
+
+  Definition exprImp2Riscv(s: @ExprImp.stmt wlit var): list (@Instruction wlit wjimm var) :=
+    let ngs := freshNameGenState (ExprImp.allVars_stmt s) in
+    let (sFlat, ngs') := flattenStmt ngs s in
+    FlatToRiscv.compile_stmt sFlat.
+
+  Definition evalH := @ExprImp.eval_stmt w wlit wdiff eq_refl var state stateMap.
+
+  Definition evalL(fuel: nat)(insts: list Instruction): RiscvMachine :=
+    execState (run (w_lbound := w_lbound) fuel) (initialRiscvMachine insts).
+
+  Lemma exprImp2Riscv_correct: forall sH instsL fuelH finalH,
+    ExprImp.stmt_size sH * 64 < pow2 wlit ->
+    exprImp2Riscv sH = instsL ->
+    eval_stmt_H fuelH empty sH = Some finalH ->
+    exists fuelL,
+      forall resVar res,
+      get finalH resVar = Some res ->
+      (evalL fuelL instsL).(registers) resVar = res.
+  Proof.
+    introv B C EvH.
+    unfold exprImp2Riscv in C.
+    destruct_one_match_hyp.
+    unfold eval_stmt_H in EvH.
+    pose proof flattenStmt_correct as P.
+    specialize (P fuelH sH s finalH).
+    destruct P as [fuelM [finalM [EvM GM]]].
+    - unfold ExprImp2FlatImp. rewrite E. reflexivity.
+    - unfold eval_stmt_H. apply EvH.
+    - pose proof  (@FlatToRiscv.compile_stmt_correct
+        wlit wdiff wjimm w_lbound wlit_bound wjimm_bound var eq_var_dec) as P.
+      specialize P with (2 := C).
+      specialize P with (2 := EvM).
+      destruct P as [fuelL P].
+      + pose proof @flattenStmt_size as D1.
+        specialize D1 with (1 := E).
+        clear -B D1.
+        omega.
+      + exists fuelL.
+        introv G.
+        apply P.
+        apply GM.
+        apply G.
+  Qed.
+
+End Pipeline.
